\documentclass[a4paper,11pt,fleqn]{article}
\usepackage[chap=4]{../ex}

\begin{document}

\maketitle
\subsection{4.12.}
Inverse map is obtained as
\begin{equation}
    \left\lbrace\begin{array}{c}
        x' = x - 1.6y'(1-y'^2) \\
        y' = y + 1.6x(1-x^2)
    \end{array}\right. .
\end{equation}
The jacobian of $f$ is given as 
\begin{equation}
    Df(x,y) = \left(\begin{array}{cc}
        1 & 1.6(1-3y^2) \\
        -1.6(1-3x'^2) & 1-1.6^2(1-3y^2)(1-3x'^2)
    \end{array} \right). 
\end{equation}
$f$ is injective and $\mathop{\rm det}{(Df(x,y))}\equiv 1$, so $f$ is area-preserving. 
The fixed points $(x_*,y_*)$s satisfy simultaneous equations $y(1-y^2)=0, x(1-x^2)=0$, so $(x_*,y_*) \in \{0,1,-1\}^2$. If $\mathop{\rm tr}{(Df(x_*,y_*))}^2-4 \mathop{\rm det}{(Df(x_*,y_*))} = \mathop{\rm tr}{(Df(x_*,y_*))}^2 - 4 > 0$, $f$ is hyperbolic at the fixed point and non-hyperbolic otherwise. 
\begin{align}
    &\mathop{\rm tr}{(Df(x_*,y_*))}^2 - 4 = -1.6^2\times 4(1-3y_*^2)(1-3x_*^2) + 1.6^4(1-3y_*^2)^2(1-3x_*^2)^2 > 0 \nonumber \\
    &\Leftrightarrow g(x_*,y_*):= 4 -1.6^2(1-3y_*^2)(1-3x_*^2) \left\lbrace \begin{array}{cc}
        <0 & \text{if} \ |x_*|+|y_*|\neq 1 \\
        >0 & \text{otherwise}
    \end{array}\right. . \ (\because x_*, y_* \text{ are not irrational} )
\end{align}
We evaluate $g$ on the fixed points as 
\begin{align}
    g(0,0) = 4 - 1.6^2 >0 \nonumber \\
    g(0,\pm 1) = g(\pm 1,0) = 4+1.6^2\times2 >0 \nonumber \\
    g(\pm 1,\pm 1) = 4-4\times 1.6^2 <0 .
\end{align}
Therefore, $(0,0)$ is non-hyperbolic and the others are hyperbolic. 
\hruleskip

\subsection{4.20.}
We take inner product with $\xi-\eta$ on both sides of $\xi=\eta+(\xi-\eta)$ as 
\begin{align}
    &(\xi-\eta,\xi) = (\xi-\eta,\eta)+||\xi-\eta||^2 \nonumber \\
    &\Leftrightarrow 2-2\cos{\theta} = ||\xi-\eta||^2. \label{eq: thetaineq}
\end{align}
Then 
\begin{align}
    &||A\xi - A\eta||^2 = ||A\xi||^2+||A\eta||^2-2(A\xi,A\eta) \ge ||A\xi||^2+||A\eta||^2-2||A\xi||\cdot||A\eta|| = (\varrho^{-1}-\varrho)^2 \\
    &||A\xi - A\eta||^2 \le ||A||_2^2||\xi-\eta||^2=||A||_2^2(2-2\cos{\theta}) \ (\because \text{Eq.~}(\ref{eq: thetaineq})). 
\end{align}
Thus the desired inequality is derived. 
\hruleskip

\subsection{4.21.}
Let $v=\xi+\eta, \xi \in E^{\rm u}, \eta \in E^{\rm s}$. Let $\lambda_{\rm s}, C_{\rm s}$ (resp. $\lambda_{\rm u}, C_{\rm u}$) be constants which make all tangent vectors in $E^{\rm s}$ (resp. $E^{\rm u}$) stable and define $C = \max{(C_{\rm s},C_{\rm u})}$ and $\lambda = \max{(\lambda_{\rm s},\lambda_{\rm u})}$. Also let $P_{\rm s}, P_{\rm u}$ be projections onto $E^{\rm s}, E^{\rm u}$. 
\begin{align}
    &\langle v,v \rangle \ge ||\xi||^2 + ||\eta||^2 \ge ||\xi+\eta||^2 = (v,v), \\
    &\langle v,v \rangle \le \frac{C_{\rm s}^2||\xi||^2}{1-\lambda_{\rm s}^{2\epsilon}} + \frac{C_{\rm u}^2||\eta||^2}{1-\lambda_{\rm u}^{2\epsilon}} \le \frac{C^2}{1-\lambda^{2\epsilon}}(||\xi||^2 + ||\eta||^2) = \frac{C^2}{1-\lambda^{2\epsilon}}(||P_{\rm u}v||^2 + ||P_{\rm s}v||^2) \nonumber \\
    &\le \frac{C^2}{1-\lambda^{2\epsilon}}(||P_{\rm u}||_2^2 + ||P_{\rm s}||_2^2)(v,v). 
\end{align}
Thus we can take $D = \max{\left(1,\frac{C^2}{1-\lambda^{2\epsilon}}(||P_{\rm u}||_2^2 + ||P_{\rm s}||_2^2)\right)}$.
\hruleskip

\subsection{4.22.(WIP)}
$C^2$ regularity of $f$ gives rise to $||Q(x)||\le \mathcal{O}(1)||x||^2$, which follows from the mean value form of the remainder of the Taylor's theorem. 

\end{document}